iso_dh/game.v
@@ -8,6 +8,7 @@ From iris.heap_lang.lib Require Import par assert ticket_lock.
 From cryptis Require Import lib cryptis primitives tactics gmeta.
 From cryptis Require Import role session iso_dh.
 From cryptis.lib Require Import term_set.
+From cryptis.primitives Require Import attacker.
 
 Set Implicit Arguments.
 Unset Strict Implicit.
@@ -282,8 +283,8 @@ iIntros "%set #set". wp_pures.
 by wp_apply wp_do_resp_loop => //.
 Qed.
 
-Definition game : val := λ: "mkchan",
-  let: "c"   := "mkchan" #() in
+Definition game : val := λ: <>,
+  let: "c"   := init_network #() in
   let: "skI" := mksigkey #() in
   let: "skR" := mksigkey #() in
   let: "vkI" := vkey "skI" in
@@ -295,20 +296,18 @@ Definition game : val := λ: "mkchan",
   Fork (do_resp "c" "compromised" "skR" "vkI");;
   Fork (compromise_long_term_keys "c" "compromised" "skI" "skR").
 
-Lemma wp_game (mkchan : val) :
-  {{{ True }}} mkchan #() {{{ v, RET v; channel v }}} -∗
+Lemma wp_game :
   cryptis_ctx -∗
   seal_pred_token ⊤ -∗
   key_pred_token (⊤ ∖ ↑nroot.@"keys") -∗
   honest 0 ∅ -∗
   ●Ph 0 -∗
-  WP game mkchan {{ _, True }}.
+  WP game #() {{ _, True }}.
 Proof.
-iIntros "wp_mkchan #ctx enc_tok key_tok _ _"; rewrite /game; wp_pures.
+iIntros "#ctx enc_tok key_tok _ _"; rewrite /game; wp_pures.
 iMod (iso_dh_ctx_alloc N with "enc_tok") as "#?" => //.
-wp_bind (mkchan _); iApply "wp_mkchan" => //.
-iIntros "!> %c #cP".
-wp_pures. wp_apply (wp_mksigkey with "[]"); eauto.
+wp_apply wp_init_network => //. iIntros "%c #cP". wp_pures.
+wp_apply (wp_mksigkey with "[]"); eauto.
 iIntros "%skI #p_vkI s_skI tokenI". wp_pures.
 wp_pures. wp_apply (wp_mksigkey with "[]"); eauto.
 iIntros "%skR #p_vkR s_skR tokenR". wp_pures.
@@ -331,19 +330,15 @@ End Game.
 Definition F : gFunctors :=
   #[heapΣ; spawnΣ; cryptisΣ; tlockΣ].
 
-Lemma iso_dh_secure (mkchan : val) σ₁ σ₂ (v : val) t₂ e₂ :
-  (∀ `{!heapGS Σ, !cryptisGS Σ},
-     ⊢ {{{ True }}} mkchan #() {{{ c, RET c; channel c}}}) →
-  rtc erased_step ([game mkchan], σ₁) (t₂, σ₂) →
+Lemma iso_dh_secure σ₁ σ₂ (v : val) t₂ e₂ :
+  rtc erased_step ([game #()], σ₁) (t₂, σ₂) →
   e₂ ∈ t₂ →
   not_stuck e₂ σ₂.
 Proof.
 have ? : heapGpreS F by apply _.
-move=> wp_mkchan.
 apply (adequate_not_stuck NotStuck _ _ (λ v _, True)) => //.
 apply: heap_adequacy.
 iIntros (?) "?".
 iMod (cryptisGS_alloc _) as (?) "(#ctx & enc_tok & key_tok & ? & hon & phase)".
-iApply (wp_game with "[] ctx [enc_tok] [key_tok] [hon]") => //.
-iApply wp_mkchan.
+by iApply (wp_game with "ctx [enc_tok] [key_tok] [hon]") => //.
 Qed.
