cryptis.v
@@ -4,6 +4,7 @@ From iris.algebra Require Import agree auth gset gmap list reservation_map excl.
 From iris.algebra Require Import functions.
 From iris.base_logic.lib Require Import saved_prop invariants.
 From iris.heap_lang Require Import notation proofmode.
+From iris.heap_lang.lib Require Import ticket_lock.
 From cryptis Require Import lib gmeta nown.
 From cryptis.core Require Export term term_meta minted public phase.
 
@@ -17,24 +18,28 @@ Class cryptisGpreS Σ := CryptisGPreS {
   cryptisGpreS_term_meta : term_metaGpreS Σ;
   cryptisGpreS_public : publicGpreS Σ;
   cryptisGpreS_phase : phaseGpreS Σ;
+  cryptisGpreS_tlock : tlockG Σ;
 }.
 
 Local Existing Instance cryptisGpreS_term_meta.
 Local Existing Instance cryptisGpreS_public.
 Local Existing Instance cryptisGpreS_phase.
+Local Existing Instance cryptisGpreS_tlock.
 
 Class cryptisGS Σ := CryptisGS {
   cryptisGS_term_meta : term_metaGS Σ;
   cryptisGS_public : publicGS Σ;
   cryptisGS_phase : phaseGS Σ;
+  cryptisGS_tlock : tlockG Σ;
 }.
 
 Global Existing Instance cryptisGS_term_meta.
 Global Existing Instance cryptisGS_public.
 Global Existing Instance cryptisGS_phase.
+Local Existing Instance cryptisGS_tlock.
 
 Definition cryptisΣ : gFunctors :=
-  #[term_metaΣ; publicΣ; phaseΣ].
+  #[term_metaΣ; publicΣ; phaseΣ; tlockΣ].
 
 Global Instance subG_cryptisGpreS Σ : subG cryptisΣ Σ → cryptisGpreS Σ.
 Proof. solve_inG. Qed.
@@ -89,6 +94,6 @@ move=> ?; iStartProof.
 iMod term_metaGS_alloc as "[% #?]".
 iMod publicGS_alloc as "(% & #? & ? & ? & ?)".
 iMod phaseGS_alloc as "(% & #? & ? & ?)".
-iExists (CryptisGS _ _ _). iFrame. iModIntro.
+iExists (CryptisGS _ _ _ _). iFrame. iModIntro.
 by do !iSplit => //.
 Qed.
