primitives/attacker.v
@@ -1,0 +1,212 @@
+From mathcomp Require Import ssreflect.
+From mathcomp Require order.
+From stdpp Require Import gmap.
+From iris.algebra Require Import agree auth gset gmap reservation_map.
+From iris.base_logic.lib Require Import invariants saved_prop.
+From iris.program_logic Require Import atomic.
+From iris.heap_lang Require Import notation proofmode.
+From iris.heap_lang.lib Require Import nondet_bool ticket_lock.
+From cryptis Require Import lib term cryptis.
+From cryptis.primitives Require Import notations comp simple.
+
+Set Implicit Arguments.
+Unset Strict Implicit.
+Unset Printing Implicit Defensive.
+
+Definition add_int : val := λ: "c",
+  let: "n" := nondet_int #() in
+  send "c" (tint "n").
+
+Definition add_pair : val := λ: "c",
+  let: "t1" := recv "c" in
+  let: "t2" := recv "c" in
+  send "c" (tuple "t1" "t2").
+
+Definition add_proj : val := λ: "c",
+  let: "t" := recv "c" in
+  match: untuple "t" with
+    NONE => #()
+  | SOME "v" => send "c" (Fst "v");; send "c" (Snd "v")
+  end.
+
+Definition add_nonce : val := λ: "c",
+  send "c" (mknonce #()).
+
+Definition add_keys : val := λ: "c",
+  let: "t" := recv "c" in
+  send "c" (key Seal "t");;
+  send "c" (key Open "t").
+
+Definition add_seal : val := λ: "c",
+  let: "t1" := recv "c" in
+  let: "t2" := recv "c" in
+  send "c" (seal "t1" "t2").
+
+Definition add_open : val := λ: "c",
+  let: "t1" := recv "c" in
+  let: "t2" := recv "c" in
+  match: open "t1" "t2" with
+    NONE => #()
+  | SOME "t" => send "c" "t"
+  end.
+
+Definition add_hash : val := λ: "c",
+  let: "t" := recv "c" in
+  send "c" (hash "t").
+
+Definition add_exp : val := λ: "c",
+  let: "t1" := recv "c" in
+  let: "t2" := recv "c" in
+  send "c" (texp "t1" "t2").
+
+Definition init_attacker : val := rec: "loop" "c" :=
+  Fork (
+    add_int "c";;
+    add_pair "c";;
+    add_proj "c";;
+    add_nonce "c";;
+    add_keys "c";;
+    add_seal "c";;
+    add_open "c";;
+    add_hash "c";;
+    add_exp "c";;
+    "loop" "c").
+
+Definition init_network : val := λ: <>,
+  let: "c" := mkchannel #() in
+  init_attacker "c";;
+  "c".
+
+Section Proofs.
+
+Context `{!heapGS Σ, !cryptisGS Σ}.
+
+Lemma wp_add_int c :
+  {{{ channel c }}} add_int c {{{ RET #(); True }}}.
+Proof.
+iIntros "%Ψ #c post".
+wp_lam. wp_apply wp_nondet_int. iIntros "%n". wp_pures.
+wp_apply wp_tint. wp_apply wp_send => //.
+  by rewrite public_TInt.
+by iApply "post".
+Qed.
+
+Lemma wp_add_pair c :
+  {{{ channel c }}} add_pair c {{{ RET #(); True }}}.
+Proof.
+iIntros "%Ψ #c post". wp_lam.
+wp_apply wp_recv => //. iIntros "%t1 #p_t1". wp_pures.
+wp_apply wp_recv => //. iIntros "%t2 #p_t2". wp_pures.
+wp_apply wp_tuple. wp_apply wp_send => //.
+- by iApply public_TPair; eauto.
+- by iApply "post".
+Qed.
+
+Lemma wp_add_proj c :
+  {{{ channel c }}} add_proj c {{{ RET #(); True }}}.
+Proof.
+iIntros "%Ψ #c post". wp_lam.
+wp_apply wp_recv => //. iIntros "%t #p_t". wp_pures.
+wp_apply wp_untuple.
+case: t => *; wp_pures; try by iApply "post".
+rewrite public_TPair. iDestruct "p_t" as "[??]".
+wp_apply wp_send => //. wp_pures.
+wp_apply wp_send => //. by iApply "post".
+Qed.
+
+Lemma wp_add_nonce c :
+  {{{ cryptis_ctx ∗ channel c }}} add_nonce c {{{ RET #(); True }}}.
+Proof.
+iIntros "%Ψ [#? #c] post". wp_lam.
+wp_apply (wp_mknonce (λ _, True)%I (λ _, True)%I) => //.
+iIntros "%t _ _ #p_t _ _".
+wp_apply wp_send => //.
+- by iApply "p_t".
+- by iApply "post".
+Qed.
+
+Lemma wp_add_keys c :
+  {{{ channel c }}} add_keys c {{{ RET #(); True }}}.
+Proof.
+iIntros "%Ψ #c post". wp_lam.
+wp_apply wp_recv => //. iIntros "%t #p_t". wp_pures.
+wp_apply wp_key => //.
+wp_apply wp_send => //; first by iApply public_TKey; eauto.
+wp_pures. wp_apply wp_key.
+wp_apply wp_send => //; first by iApply public_TKey; eauto.
+by iApply "post".
+Qed.
+
+Lemma wp_add_seal c :
+  {{{ channel c }}} add_seal c {{{ RET #(); True }}}.
+Proof.
+iIntros "%Ψ #c post". wp_lam.
+wp_apply wp_recv => //. iIntros "%t1 #p_t1". wp_pures.
+wp_apply wp_recv => //. iIntros "%t2 #p_t2". wp_pures.
+wp_apply wp_seal. wp_apply wp_send => //.
+- by iApply public_TSeal; eauto.
+- by iApply "post".
+Qed.
+
+Lemma wp_add_open c :
+  {{{ channel c }}} add_open c {{{ RET #(); True }}}.
+Proof.
+iIntros "%Ψ #c post". wp_lam.
+wp_apply wp_recv => //. iIntros "%t1 #p_t1". wp_pures.
+wp_apply wp_recv => //. iIntros "%t2 #p_t2". wp_pures.
+wp_apply wp_open.
+case: Spec.openP => [ {}t1 {}t2 -> ->|]; wp_pures; last by iApply "post".
+wp_apply wp_send => //; last by iApply "post".
+rewrite public_TSeal.
+iDestruct "p_t2" as "[[_ ?]|(_ & _ & p_t2)]" => //.
+by iApply "p_t2".
+Qed.
+
+Lemma wp_add_hash c :
+  {{{ channel c }}} add_hash c {{{ RET #(); True }}}.
+Proof.
+iIntros "%Ψ #c post". wp_lam.
+wp_apply wp_recv => //. iIntros "%t #p_t". wp_pures.
+wp_apply wp_hash.
+wp_apply wp_send => //; last by iApply "post".
+by rewrite public_THash; eauto.
+Qed.
+
+Lemma wp_add_exp c :
+  {{{ channel c }}} add_exp c {{{ RET #(); True }}}.
+Proof.
+iIntros "%Ψ #c post". wp_lam.
+wp_apply wp_recv => //. iIntros "%t1 #p_t1". wp_pures.
+wp_apply wp_recv => //. iIntros "%t2 #p_t2". wp_pures.
+wp_apply wp_texp. wp_apply wp_send => //; last by iApply "post".
+by iApply public_TExp.
+Qed.
+
+Lemma wp_init_attacker c :
+  {{{ cryptis_ctx ∗ channel c }}} init_attacker c {{{ RET #(); True }}}.
+Proof.
+iLöb as "IH".
+iIntros "%Ψ [#? #?] post".
+wp_rec. wp_apply wp_fork; last by iApply "post".
+wp_apply wp_add_int => //. iIntros "_". wp_pures.
+wp_apply wp_add_pair => //. iIntros "_". wp_pures.
+wp_apply wp_add_proj => //. iIntros "_". wp_pures.
+wp_apply wp_add_nonce => //; eauto. iIntros "_". wp_pures.
+wp_apply wp_add_keys => //. iIntros "_". wp_pures.
+wp_apply wp_add_seal => //. iIntros "_". wp_pures.
+wp_apply wp_add_open => //. iIntros "_". wp_pures.
+wp_apply wp_add_hash => //. iIntros "_". wp_pures.
+wp_apply wp_add_exp => //. iIntros "_". wp_pures.
+by wp_apply "IH"; eauto.
+Qed.
+
+Lemma wp_init_network :
+  {{{ cryptis_ctx }}} init_network #() {{{ c, RET c; channel c }}}.
+Proof.
+iIntros "%Ψ #ctx post".
+wp_lam. wp_apply wp_mkchannel. iIntros "%c #cP". wp_pures.
+wp_apply wp_init_attacker; eauto. iIntros "_". wp_pures.
+by iApply "post".
+Qed.
+
+End Proofs.
